src/program_proof/memkv/memkv_put_proof.v
@@ -200,8 +200,7 @@ Proof.
     assert (∃ b, shardMapping !! int.nat sid = Some b) as [? ?].
     {
       eapply list_lookup_lt.
-      rewrite HshardMapLength.
-      rewrite /sid /shardOfC /uNSHARD.
+      move: HshardMapLength. rewrite /sid /shardOfC /uNSHARD.
       word.
     }
     wp_apply (typed_slice.wp_SliceGet with "[$HshardMap_sl]").
@@ -211,7 +210,7 @@ Proof.
     iIntros "HshardMap_sl".
     wp_pures.
 
-    assert (int.Z seqno < int.Z args.(PR_Seq))%Z as HseqFresh.
+    assert (int.Z seqno < int.Z args.(PR_Seq)) as HseqFresh.
     {
       simpl.
       destruct ok.
